BitVector with all bitwise proofs

lib/hst/FStar.BitVector.fst
@@ -7,12 +7,12 @@ open FStar.Seq
 type bv_t (n:nat) = vec:seq bool{length vec = n}
 
 (* Constants *)
-val zero_vec: n:pos -> Tot (bv_t n)
-let zero_vec n = create n false
-val elem_vec: n:pos -> i:nat{i < n} -> Tot (bv_t n)
-let elem_vec n i = upd (create n false) i true
-val ones_vec: n:pos -> Tot (bv_t n)
-let ones_vec n = create n true
+val zero_vec: #n:pos -> Tot (bv_t n)
+let zero_vec #n = create n false
+val elem_vec: #n:pos -> i:nat{i < n} -> Tot (bv_t n)
+let elem_vec #n i = upd (create n false) i true
+val ones_vec: #n:pos -> Tot (bv_t n)
+let ones_vec #n = create n true
 
 (* Bitwise operators *)
 val logand_vec: #n:pos -> a:bv_t n -> b:bv_t n -> Tot (bv_t n)
@@ -68,6 +68,44 @@ let rec lognot_vec_definition #n a i =
   if i = 0 then ()
   else lognot_vec_definition #(n - 1) (slice a 1 n) (i - 1)
 
+(* Shift operators *)
+val shift_left_vec: #n:pos -> a:bv_t n -> s:nat -> Tot (bv_t n)
+let shift_left_vec #n a s =
+  if s >= n then zero_vec #n
+  else if s = 0 then a
+  else append (slice a s n) (zero_vec #s)
+  
+val shift_right_vec: #n:pos -> a:bv_t n -> s:nat -> Tot (bv_t n)
+let shift_right_vec #n a s =
+  if s >= n then zero_vec #n
+  else if s = 0 then a
+  else append (zero_vec #s) (slice a 0 (n - s))
+
+(* Shift operators lemmas *)
+val shift_left_vec_lemma_1: #n:pos -> a:bv_t n -> s:nat -> i:nat{i < n && i >= n - s} ->
+  Lemma (requires True)
+        (ensures index (shift_left_vec #n a s) i = false)
+	[SMTPat (index (shift_left_vec #n a s) i)]
+let shift_left_vec_lemma_1 #n a s i = ()
+
+val shift_left_vec_lemma_2: #n:pos -> a:bv_t n -> s:nat -> i:nat{i < n && i < n - s} ->
+  Lemma (requires True)
+        (ensures index (shift_left_vec #n a s) i = index a (i + s))
+	[SMTPat (index (shift_left_vec #n a s) i)]
+let shift_left_vec_lemma_2 #n a s i = ()
+
+val shift_right_vec_lemma_1: #n:pos -> a:bv_t n -> s:nat -> i:nat{i < n && i < s} ->
+  Lemma (requires True)
+        (ensures index (shift_right_vec #n a s) i = false)
+	[SMTPat (index (shift_right_vec #n a s) i)]
+let shift_right_vec_lemma_1 #n a s i = ()
+
+val shift_right_vec_lemma_2: #n:pos -> a:bv_t n -> s:nat -> i:nat{i < n && i >= s} ->
+  Lemma (requires True)
+        (ensures index (shift_right_vec #n a s) i = index a (i - s))
+	[SMTPat (index (shift_right_vec #n a s) i)]
+let shift_right_vec_lemma_2 #n a s i = ()
+
 
 (* Define bitwise operators for type uint. *)
 open FStar.UInt.BV
@@ -84,13 +122,13 @@ let rec from_vec #n vec =
   if n = 0 then 0
   else 2 * from_vec #(n - 1) (slice vec 1 n) + (if index vec 0 then 1 else 0)
 
-val to_vec_bijection_lemma: #n:nat -> a:uint_t n -> b:uint_t n ->
+val to_vec_lemma: #n:nat -> a:uint_t n -> b:uint_t n ->
   Lemma (requires equal (to_vec a) (to_vec b)) (ensures a = b)
-let rec to_vec_bijection_lemma #n a b =
+let rec to_vec_lemma #n a b =
   if n = 0 then () else begin
     assert(equal (slice (to_vec b) 1 n) (to_vec #(n - 1) (b / 2)));
     assert(equal (slice (to_vec a) 1 n) (to_vec #(n - 1) (a / 2)));
-    to_vec_bijection_lemma #(n - 1) (a / 2) (b / 2);
+    to_vec_lemma #(n - 1) (a / 2) (b / 2);
     assert(a % 2 = (if index (to_vec a) 0 then 1 else 0));
     assert(b % 2 = (if index (to_vec b) 0 then 1 else 0));
     assert(a % 2 = b % 2)
@@ -110,11 +148,61 @@ let inverse_vec_lemma #n vec = ()
 val inverse_num_lemma: #n:nat -> num:uint_t n ->
   Lemma (requires True) (ensures num = from_vec (to_vec num))
         [SMTPat (from_vec (to_vec num))]
-let inverse_num_lemma #n num = to_vec_bijection_lemma #n num (from_vec (to_vec num))
+let inverse_num_lemma #n num = to_vec_lemma #n num (from_vec (to_vec num))
 
-val from_vec_bijection_lemma: #n:nat -> a:bv_t n -> b:bv_t n ->
+val from_vec_lemma: #n:nat -> a:bv_t n -> b:bv_t n ->
   Lemma (requires from_vec a = from_vec b) (ensures equal a b)
-let from_vec_bijection_lemma #n a b = inverse_vec_lemma a; inverse_vec_lemma b
+let from_vec_lemma #n a b = inverse_vec_lemma a; inverse_vec_lemma b
+
+
+(* Relations between constants in BitVector and in UInt. *)
+val zero_to_vec_lemma: #n:pos -> i:nat{i < n} ->
+  Lemma (requires True) (ensures index (to_vec (zero #n)) i = index (zero_vec #n) i)
+        [SMTPat (index (to_vec (zero #n)) i)]
+let rec zero_to_vec_lemma #n i =
+  if i = 0 then () else zero_to_vec_lemma #(n - 1) (i - 1)
+
+val zero_from_vec_lemma: #n:pos ->
+  Lemma (requires True) (ensures from_vec (zero_vec #n) = zero #n)
+        [SMTPat (from_vec (zero_vec #n))]
+let zero_from_vec_lemma #n = to_vec_lemma (from_vec (zero_vec #n)) (zero #n)
+
+val one_to_vec_lemma: #n:pos -> i:nat{i < n} ->
+  Lemma (requires True)
+        (ensures index (to_vec (one #n)) i = index (elem_vec #n 0) i)
+	[SMTPat (index (to_vec (one #n)) i)]
+let one_to_vec_lemma #n i =
+  if i = 0 then () else zero_to_vec_lemma #n i
+
+val pow2_to_vec_lemma: #n:pos -> p:nat{p < n} -> i:nat{i < n} ->
+  Lemma (requires True)
+        (ensures index (to_vec (pow2_n #n p)) i = index (elem_vec #n p) i)
+	[SMTPat (index (to_vec (pow2_n #n p)) i)]
+let rec pow2_to_vec_lemma #n p i =
+  if i = 0 then () 
+  else if p = 0 then one_to_vec_lemma #n i
+  else pow2_to_vec_lemma #(n - 1) (p - 1) (i - 1)
+
+val pow2_from_vec_lemma: #n:pos -> p:nat{p < n} ->
+  Lemma (requires True) (ensures from_vec (elem_vec #n p) = pow2_n #n p)
+        [SMTPat (from_vec (elem_vec #n p))]
+let pow2_from_vec_lemma #n p = to_vec_lemma (from_vec (elem_vec #n p)) (pow2_n #n p)
+
+val ones_to_vec_lemma: #n:pos -> i:nat{i < n} ->
+  Lemma (requires True)
+        (ensures index (to_vec (ones #n)) i = index (ones_vec #n) i)
+	[SMTPat (index (to_vec (ones #n)) i)]
+let rec ones_to_vec_lemma #n i =
+  if i = 0 then () else begin 
+     pow2_exp_1 i (n - i);
+     division_definition (pow2 n - 1) (pow2 i) (pow2 (n - i) - 1);
+     ones_to_vec_lemma #(n - 1) (i - 1)
+  end
+
+val ones_from_vec_lemma: #n:pos ->
+  Lemma (requires True) (ensures from_vec (ones_vec #n) = ones #n)
+        [SMTPat (from_vec (ones_vec #n))]
+let ones_from_vec_lemma #n = to_vec_lemma (from_vec (ones_vec #n)) (ones #n)
 
 
 (* (nth a i) returns a boolean indicating the i-th bit of a. *)
@@ -126,32 +214,32 @@ val nth_lemma: #n:pos -> a:uint_t n -> b:uint_t n ->
         (ensures a = b)
 let nth_lemma #n a b =
   assert(forall (i:nat{i < n}). index (to_vec #n a) i = index (to_vec #n b) i);
-  to_vec_bijection_lemma a b
+  to_vec_lemma a b
 
 (* Lemmas for constants *)
 val zero_nth_lemma: #n:pos -> i:nat{i < n} ->
-  Lemma (requires True) (ensures nth (zero n) i = false)
-        [SMTPat (nth (zero n) i)]
-let rec zero_nth_lemma #n i =
-  if i = 0 then () else zero_nth_lemma #(n - 1) (i - 1)
+  Lemma (requires True) (ensures nth (zero #n) i = false)
+        [SMTPat (nth (zero #n) i)]
+let rec zero_nth_lemma #n i = ()
+
+val pow2_nth_lemma: #n:pos -> p:nat{p < n} -> i:nat{i < n} ->
+  Lemma (requires True)
+        (ensures (i = p ==> nth (pow2_n #n p) i = true) /\
+	         (i > p ==> nth (pow2_n #n p) i = false))
+        [SMTPat (nth (pow2_n #n p) i)]
+let pow2_nth_lemma #n p i = ()
 
 val one_nth_lemma: #n:pos -> i:nat{i < n} ->
   Lemma (requires True)
-        (ensures (i = 0 ==> nth (one n) i = true) /\
-	         (i > 0 ==> nth (one n) i = false))
-        [SMTPat (nth (one n) i)]
-let one_nth_lemma #n i =
-  if i = 0 then () else zero_nth_lemma #(n - 1) (i - 1)
+        (ensures (i = 0 ==> nth (one #n) i = true) /\
+	         (i > 0 ==> nth (one #n) i = false))
+        [SMTPat (nth (one #n) i)]
+let one_nth_lemma #n i = ()
 
 val ones_nth_lemma: #n:pos -> i:nat{i < n} ->
-  Lemma (requires True) (ensures (nth (ones n) i) = true)
-        [SMTPat (nth (ones n) i)]
-let rec ones_nth_lemma #n i =
-  if i = 0 then () else begin
-    pow2_exp_1 1 (n - 1);
-    division_definition (pow2 n - 1) (pow2 1) (pow2 (n - 1) - 1);
-    ones_nth_lemma #(n - 1) (i - 1)
-  end
+  Lemma (requires True) (ensures (nth (ones #n) i) = true)
+        [SMTPat (nth (ones #n) i)]
+let rec ones_nth_lemma #n i = ()
 
 (* Bitwise operators *)
 val logand: #n:pos -> a:uint_t n -> b:uint_t n -> Tot (uint_t n)
@@ -202,12 +290,12 @@ val logand_self: #n:pos -> a:uint_t n ->
 let logand_self #n a = nth_lemma #n (logand #n a a) a
 
 val logand_lemma_1: #n:pos -> a:uint_t n -> 
-  Lemma (requires True) (ensures (logand #n a (zero n) = zero n))
-let logand_lemma_1 #n a = nth_lemma #n (logand #n a (zero n)) (zero n)
+  Lemma (requires True) (ensures (logand #n a (zero #n) = zero #n))
+let logand_lemma_1 #n a = nth_lemma #n (logand #n a (zero #n)) (zero #n)
 
 val logand_lemma_2: #n:pos -> a:uint_t n -> 
-  Lemma (requires True) (ensures (logand #n a (ones n) = a))
-let logand_lemma_2 #n a = nth_lemma #n (logand #n a (ones n)) a
+  Lemma (requires True) (ensures (logand #n a (ones #n) = a))
+let logand_lemma_2 #n a = nth_lemma #n (logand #n a (ones #n)) a
 
 (* Bitwise XOR operator *)
 val logxor_commutative: #n:pos -> a:uint_t n -> b:uint_t n ->
@@ -219,16 +307,16 @@ val logxor_associative: #n:pos -> a:uint_t n -> b:uint_t n -> c:uint_t n ->
 let logxor_associative #n a b c = nth_lemma #n (logxor #n (logxor #n a b) c) (logxor #n a (logxor #n b c))
 
 val logxor_self: #n:pos -> a:uint_t n ->
-  Lemma (requires True) (ensures (logxor #n a a = zero n))
-let logxor_self #n a = nth_lemma #n (logxor #n a a) (zero n)
+  Lemma (requires True) (ensures (logxor #n a a = zero #n))
+let logxor_self #n a = nth_lemma #n (logxor #n a a) (zero #n)
 
 val logxor_lemma_1: #n:pos -> a:uint_t n -> 
-  Lemma (requires True) (ensures (logxor #n a (zero n) = a))
-let logxor_lemma_1 #n a = nth_lemma #n (logxor #n a (zero n)) a
+  Lemma (requires True) (ensures (logxor #n a (zero #n) = a))
+let logxor_lemma_1 #n a = nth_lemma #n (logxor #n a (zero #n)) a
 
 val logxor_lemma_2: #n:pos -> a:uint_t n -> 
-  Lemma (requires True) (ensures (logxor #n a (ones n) = lognot #n a))
-let logxor_lemma_2 #n a = nth_lemma #n (logxor #n a (ones n)) (lognot #n a)
+  Lemma (requires True) (ensures (logxor #n a (ones #n) = lognot #n a))
+let logxor_lemma_2 #n a = nth_lemma #n (logxor #n a (ones #n)) (lognot #n a)
 
 (* Bitwise OR operators *)
 val logor_commutative: #n:pos -> a:uint_t n -> b:uint_t n ->
@@ -245,12 +333,12 @@ val logor_self: #n:pos -> a:uint_t n ->
 let logor_self #n a = nth_lemma #n (logor #n a a) a
 
 val logor_lemma_1: #n:pos -> a:uint_t n ->
-  Lemma (requires True) (ensures (logor #n a (zero n) = a))
-let logor_lemma_1 #n a = nth_lemma (logor #n a (zero n)) a
+  Lemma (requires True) (ensures (logor #n a (zero #n) = a))
+let logor_lemma_1 #n a = nth_lemma (logor #n a (zero #n)) a
 
 val logor_lemma_2: #n:pos -> a:uint_t n -> 
-  Lemma (requires True) (ensures (logor #n a (ones n) = ones n))
-let logor_lemma_2 #n a = nth_lemma (logor #n a (ones n)) (ones n)
+  Lemma (requires True) (ensures (logor #n a (ones #n) = ones #n))
+let logor_lemma_2 #n a = nth_lemma (logor #n a (ones #n)) (ones #n)
 
 (* Bitwise NOT operator *)
 val lognot_self: #n:pos -> a:uint_t n ->
@@ -258,5 +346,65 @@ val lognot_self: #n:pos -> a:uint_t n ->
 let lognot_self #n a = nth_lemma (lognot #n (lognot #n a)) a
 
 val lognot_lemma_1: #n:pos -> 
-  Lemma (requires True) (ensures (lognot #n (zero n) = ones n))
-let lognot_lemma_1 #n = nth_lemma (lognot #n (zero n)) (ones n)
+  Lemma (requires True) (ensures (lognot #n (zero #n) = ones #n))
+let lognot_lemma_1 #n = nth_lemma (lognot #n (zero #n)) (ones #n)
+
+
+(* Shift operators *)
+val shift_left: #n:pos -> a:uint_t n -> s:nat -> Tot (uint_t n)
+let shift_left #n a s = from_vec (shift_right_vec #n (to_vec #n a) s)
+val shift_right: #n:pos -> a:uint_t n -> s:nat -> Tot (uint_t n)
+let shift_right #n a s = from_vec (shift_left_vec #n (to_vec #n a) s)
+
+(* Shift operators lemmas *)
+val shift_left_lemma_1: #n:pos -> a:uint_t n -> s:nat -> i:nat{i < n && i < s} ->
+  Lemma (requires True)
+	(ensures (nth (shift_left #n a s) i = false))
+	[SMTPat (nth (shift_left #n a s) i)]
+let shift_left_lemma_1 #n a s i = ()
+val shift_left_lemma_2: #n:pos -> a:uint_t n -> s:nat -> i:nat{i < n && i >= s} ->
+  Lemma (requires True)
+        (ensures (nth (shift_left #n a s) i = nth #n a (i - s)))
+	[SMTPat (nth (shift_left #n a s) i)]
+let shift_left_lemma_2 #n a s i = ()
+val shift_right_lemma_1: #n:pos -> a:uint_t n -> s:nat -> i:nat{i < n && i >= n - s} ->
+  Lemma (requires True)
+	(ensures (nth (shift_right #n a s) i = false))
+	[SMTPat (nth (shift_right #n a s) i)]
+let shift_right_lemma_1 #n a s i = ()
+val shift_right_lemma_2: #n:pos -> a:uint_t n -> s:nat -> i:nat{i < n && i < n - s} ->
+  Lemma (requires True)
+        (ensures (nth (shift_right #n a s) i = nth #n a (i + s)))
+	[SMTPat (nth (shift_right #n a s) i)]
+let shift_right_lemma_2 #n a s i = ()
+
+(* Lemmas with shift operators and bitwise operators *)
+val shift_left_logand_lemma: #n:pos -> a:uint_t n -> b:uint_t n -> s:nat ->
+  Lemma (requires True)
+        (ensures (shift_left #n (logand #n a b) s = logand #n (shift_left #n a s) (shift_left #n b s)))
+let shift_left_logand_lemma #n a b s = nth_lemma (shift_left #n (logand #n a b) s) (logand #n (shift_left #n a s) (shift_left #n b s))
+
+val shift_right_logand_lemma: #n:pos -> a:uint_t n -> b:uint_t n -> s:nat ->
+  Lemma (requires True)
+        (ensures (shift_right #n (logand #n a b) s = logand #n (shift_right #n a s) (shift_right #n b s)))
+let shift_right_logand_lemma #n a b s = nth_lemma (shift_right #n (logand #n a b) s) (logand #n (shift_right #n a s) (shift_right #n b s))
+
+val shift_left_logxor_lemma: #n:pos -> a:uint_t n -> b:uint_t n -> s:nat ->
+  Lemma (requires True)
+        (ensures (shift_left #n (logxor #n a b) s = logxor #n (shift_left #n a s) (shift_left #n b s)))
+let shift_left_logxor_lemma #n a b s = nth_lemma (shift_left #n (logxor #n a b) s) (logxor #n (shift_left #n a s) (shift_left #n b s))
+
+val shift_right_logxor_lemma: #n:pos -> a:uint_t n -> b:uint_t n -> s:nat ->
+  Lemma (requires True)
+        (ensures (shift_right #n (logxor #n a b) s = logxor #n (shift_right #n a s) (shift_right #n b s)))
+let shift_right_logxor_lemma #n a b s = nth_lemma (shift_right #n (logxor #n a b) s) (logxor #n (shift_right #n a s) (shift_right #n b s))
+
+val shift_left_logor_lemma: #n:pos -> a:uint_t n -> b:uint_t n -> s:nat ->
+  Lemma (requires True)
+        (ensures (shift_left #n (logor #n a b) s = logor #n (shift_left #n a s) (shift_left #n b s)))
+let shift_left_logor_lemma #n a b s = nth_lemma (shift_left #n (logor #n a b) s) (logor #n (shift_left #n a s) (shift_left #n b s))
+
+val shift_right_logor_lemma: #n:pos -> a:uint_t n -> b:uint_t n -> s:nat ->
+  Lemma (requires True)
+        (ensures (shift_right #n (logor #n a b) s = logor #n (shift_right #n a s) (shift_right #n b s)))
+let shift_right_logor_lemma #n a b s = nth_lemma (shift_right #n (logor #n a b) s) (logor #n (shift_right #n a s) (shift_right #n b s))
